testcases/Test_Map.thy
@@ -1,0 +1,34 @@
+theory Test_Map
+  imports "../DP_Lifting"
+begin
+  
+function f :: "nat \<Rightarrow> int" where
+  "f 0 = 0"
+| "f (Suc i) = undefined [f i. i \<leftarrow> [0..<Suc i]]"
+  by pat_completeness auto
+termination
+  apply (relation "size <*mlex*> {}")
+  by (auto intro: wf_mlex mlex_less )
+    
+lemma [fundef_cong]:
+  fixes f g
+  assumes "\<And>x. x \<in> set xs \<Longrightarrow> f x = g x" "xs = ys"
+  shows   "map\<^sub>T' f xs = map\<^sub>T' g ys"  
+  using assms
+  apply (induction xs arbitrary: ys)
+  subgoal
+    by auto
+  subgoal for x xs ys
+    by (cases ys) auto
+  done
+    
+term "op ."
+term 0 (**
+    
+function f\<^sub>T :: "nat \<Rightarrow>\<^sub>T int" where
+  "f\<^sub>T 0 = \<langle>0\<rangle>"
+| "f\<^sub>T (Suc i) = undefined (map\<^sub>T' (f\<^sub>T) [0..<Suc i])"
+  by pat_completeness auto
+termination
+  apply (relation "size <*mlex*> {}")
+  by (auto intro: wf_mlex mlex_less )
